end2end: wip consistency of fetching

processor/src/processor/FetchOk.v
@@ -20,6 +20,30 @@ Require Import processor.KamiProc.
 
 Local Open Scope Z_scope.
 
+Lemma evalExpr_bit_eq_rect:
+  forall n1 n2 (Hn: n1 = n2) e,
+    evalExpr (eq_rect n1 (fun sz => Expr type (SyntaxKind (Bit sz))) e n2 Hn) =
+    eq_rect n1 Word.word (evalExpr e) n2 Hn.
+Proof.
+  intros; subst.
+  do 2 rewrite <-(Eqdep_dec.eq_rect_eq_dec eq_nat_dec).
+  reflexivity.
+Qed.
+
+Lemma ZToWord_zero:
+  forall n, ZToWord n 0 = wzero n.
+Proof.
+  destruct n; intros; [shatterer|].
+  apply wordToZ_inj.
+  rewrite wordToZ_ZToWord.
+  - rewrite wordToZ_wzero; reflexivity.
+  - split.
+    + blia.
+    + change 0 with (Z.of_nat 0).
+      apply Nat2Z.inj_lt.
+      apply NatLib.zero_lt_pow2.
+Qed.
+
 Section FetchOk.
 
   Instance W: Utility.Words := @KamiWord.WordsKami width width_cases.
@@ -31,6 +55,8 @@ Section FetchOk.
    *)
   Variable instrMemSizeLg: Z.
   Hypothesis (HinstrMemBound: 3 <= instrMemSizeLg <= width - 2).
+  Local Notation ninstrMemSizeLg := (Z.to_nat instrMemSizeLg).
+  Local Notation nwidth := (Z.to_nat width).
   Definition instrMemSize: nat := Z.to_nat (Z.pow 2 instrMemSizeLg).
   Definition dataMemSize: nat := Z.to_nat (Z.pow 2 width).
 
@@ -48,10 +74,11 @@ Section FetchOk.
     end.
 
   (* set of executable addresses in the kami processor *)
-  Definition kamiXAddrs: XAddrs := addXAddrRange (wzero _) instrMemSize nil.
+  Definition kamiXAddrs: XAddrs :=
+    addXAddrRange (wzero _) instrMemSize nil.
 
   Definition convertInstrMem (instrMem: kword instrMemSizeLg -> kword 32): mem :=
-    let keys := List.unfoldn (Word.wplus (Word.ZToWord (Z.to_nat instrMemSizeLg) 1))
+    let keys := List.unfoldn (Word.wplus (Word.ZToWord ninstrMemSizeLg 1))
                              instrMemSize (wzero _) in
     let values := List.map (fun key => word32_to_4bytes (instrMem key)) keys in
     @unchecked_store_byte_tuple_list 4 (wzero _) values map.empty.
@@ -65,79 +92,91 @@ Section FetchOk.
                     keys in
     unchecked_store_byte_tuple_list (wzero _) values map.empty.
 
-  Lemma instrMemSizeLg_bound_split:
-    (Z.to_nat width = (2 + Z.to_nat instrMemSizeLg)
-                      + (Z.to_nat width - (2 + Z.to_nat instrMemSizeLg)))%nat.
-  Proof.
-    change 2%nat with (Z.to_nat 2).
-    rewrite <-Z2Nat.inj_add by blia.
-    rewrite <-Z2Nat.inj_sub by blia.
-    rewrite <-Z2Nat.inj_add by blia.
-    f_equal; blia.
-  Qed.
-                                              
-  Definition toKamiPc (pc: kword width):
-    Word.word (2 + Z.to_nat instrMemSizeLg).
-    unfold kword in pc.
-    rewrite instrMemSizeLg_bound_split in pc.
-    exact (split1 _ _ pc).
-  Defined.
-
-  Lemma toKamiPc_wplus_distr:
-    forall w1 w2,
-      toKamiPc w1 ^+ toKamiPc w2 = toKamiPc (w1 ^+ w2).
-  Proof.
-    unfold toKamiPc; intros.
-    case TODO.
-  Qed.
+  Definition toKamiPc (pc: kword width): Word.word (2 + ninstrMemSizeLg) :=
+    split1 _ _ (eq_rec nwidth Word.word pc _ (width_inst_valid HinstrMemBound)).
 
   Lemma kamiXAddrs_In_prop:
     forall addr,
       In addr kamiXAddrs ->
-      exists saddr: Word.word 30, addr = Word.combine WO~0~0 saddr.
+      exists saddr: Word.word ninstrMemSizeLg,
+        addr =
+        eq_rect (2 + ninstrMemSizeLg + (32 - (2 + ninstrMemSizeLg)))%nat
+                Word.word
+                (Word.combine (Word.combine WO~0~0 saddr) (ZToWord _ 0))
+                nwidth
+                (eq_sym (width_inst_valid HinstrMemBound)).
   Proof.
     unfold kamiXAddrs; intros.
-    assert (exists saddr: Word.word 30,
-               wzero (BinInt.Z.to_nat width) = Word.combine WO~0~0 saddr).
-    { exists (wzero _); reflexivity. }
+    assert (exists saddr: Word.word ninstrMemSizeLg,
+               wzero (BinInt.Z.to_nat width) =
+               eq_rect (2 + ninstrMemSizeLg + (32 - (2 + ninstrMemSizeLg)))%nat
+                       Word.word
+                       (Word.combine (Word.combine WO~0~0 saddr) (ZToWord _ 0))
+                       nwidth
+                       (eq_sym (width_inst_valid HinstrMemBound))).
+    { exists (wzero _).
+      apply wordToZ_inj.
+      rewrite wordToZ_eq_rect.
+      rewrite ZToWord_zero.
+      rewrite combine_wzero.
+      rewrite (width_inst_valid HinstrMemBound).
+      reflexivity.
+    }
 
     generalize dependent (wzero (BinInt.Z.to_nat width)).
-    induction instrMemSize; simpl; intros; [exfalso; auto|].
+    induction instrMemSize; intros; [exfalso; auto|].
     destruct H; [subst; assumption|].
     eapply IHn; [eassumption|].
-    destruct H0 as [iaddr ?]; subst.
+    destruct H0 as [saddr ?]; subst.
 
-    eexists.
-    match goal with
-    | |- _ ^+ ?w = _ => replace w with (Word.combine WO~0~0 (natToWord 30 1))
-    end.
-    - simpl.
-      unfold Pos.to_nat; simpl.
-      do 2 rewrite <-wplus_WS_0'.
+    exists (saddr ^+ $1).
+    change (word.of_Z 4) with (ZToWord nwidth 4).
+    replace (ZToWord nwidth 4)
+      with (eq_rect
+              (2 + ninstrMemSizeLg + (32 - (2 + ninstrMemSizeLg)))%nat
+              Word.word (ZToWord _ 4) nwidth
+              (eq_sym (width_inst_valid HinstrMemBound))).
+    2: {
+      apply wordToZ_inj.
+      rewrite wordToZ_eq_rect.
+      rewrite (width_inst_valid HinstrMemBound).
       reflexivity.
-    - reflexivity.    
-  Qed.
+    }
+    cbv [word.add word W WordsKami wordW KamiWord.word].
+    rewrite <-eq_rect_wplus.
 
-  Lemma kamiXAddrs_toKamiPc_aligned:
-    forall addr,
-      In addr kamiXAddrs ->
-      exists iaddr, toKamiPc addr = Word.combine WO~0~0 iaddr.
-  Proof.
-    intros.
-    apply kamiXAddrs_In_prop in H.
-    destruct H as [saddr ?]; subst.
-
-    unfold toKamiPc.
+    f_equal.
     case TODO.
     
   Qed.
 
   Lemma rv32AlignAddr_toKamiPc_consistent:
-    forall addr iaddr,
-      toKamiPc addr = Word.combine WO~0~0 iaddr ->
-      addr = evalExpr (IsaRv32.rv32AlignAddr 32%nat (Z.to_nat instrMemSizeLg) type iaddr).
+    forall addr,
+      In addr kamiXAddrs ->
+      addr = evalExpr
+               (IsaRv32.rv32AlignAddr
+                  32%nat (Z.to_nat instrMemSizeLg)
+                  (width_inst_valid HinstrMemBound)
+                  type (split2 2 (Z.to_nat instrMemSizeLg) (toKamiPc addr))).
   Proof.
-    case TODO.
+    intros.
+    cbv [IsaRv32.rv32AlignAddr].
+    unfold eq_rect_r; rewrite evalExpr_bit_eq_rect.
+    cbv [evalExpr evalBinBit evalUniBit].
+    cbv [evalConstT].
+    
+    apply kamiXAddrs_In_prop in H.
+    destruct H as [saddr ?].
+    rewrite H at 1.
+    repeat f_equal.
+
+    subst.
+    unfold toKamiPc.
+    unfold eq_rec.
+    rewrite eq_rect_2.
+    rewrite split1_combine.
+    rewrite split2_combine.
+    reflexivity.
   Qed.
 
   Definition RiscvXAddrsSafe
